## The universal quantifier

### Ex.1

(a.)

```
1 (1) Fm                  A
2 (2) (x)(Fx -> Nx)       A
2 (3) Fm -> Nm            2 UE
1,2 (4) Nm                1,3 MPP
```

(b.)

```
1 (1) Nm                  A
2 (2) (x)(Nx -> !Fx)      A
2 (3) Nm -> !Fm           2 UE
1,2 (4) !Fm               1,3 MPP
```

(c.)

```
1 (1) !Fm                 A
2 (2) (x)(Ax -> Fx)       A
2 (3) Am -> Fm            2 UE
1,2 (4) !Am               1,3 MTT
```

(d.)

```
1 (1) (x)(Mx & Nx -> Sx)     A
2 (2) !Sn                    A
3 (3) Mn                     A
1 (4) Mn & Nn -> Sn          1 UE
1,2 (5) !(Mn & Nn)           1,2 MTT
1,2 (6) !Mn v !Nn            5 Demorgan
1,2 (7) Mn -> !Nn            6 derived
1,2,3 (8) !Nn                3,7 MPP
```

(e.)

```
1 (1) (x)(Fx & !Px -> Kx)    A
2 (2) Fm                     A
3 (3) !Km                    A
1 (4) Fm & !Pm -> Km         1 UE
1,3 (5) !(Fm & !Pm)          3,4 MTT
1,3 (6) !Fm v Pm             5 demorgan
1,2,3 (7) Pm                 2,6 derived
```

### Ex.2

(i.)

(a.)

`(x)(Fx -> Gx), (x)(Gx -> !Hx) => (x)(Fx -> !Hx)`

```
1 (1) (x)(Fx -> Gx)           A
2 (2) (x)(Gx -> !Hx)          A
1 (3) Fm -> Gm                1 UE
2 (4) Gm -> !Hm               2 UE
5 (5) Fm                      A
1,5 (6) Gm                    3,5 MPP
1,2,5 (7) !Hm                 3,6 MPP
1,2 (8) Fm -> !Hm             5,7 CP
1,2 (9) (x)(Fx -> !Hx)        8 UI
```

(b.)

similar to a., use MTT for `Hm -> !Gm`

(c.)

similar to b, add `DN` to `Gm`

(d.)

use to `Fm` to `Gm -> !Fm`

(e.)

```
1 (1) (x)(Fx -> Gx)         A
1 (2) Fm -> Gm              1 UE
```

can't derive to `Fm -> Fn` or `Fm -> Fo`

(f.)

```
1 (1) (x)(Fx v Gx -> Hx)     A
2 (2) (x)(!Hx)               A
1 (3) Fm v Gm -> Hm          1 UE
2 (4) !Hm                    2 UE
1,2 (5) !(Fm v Gm)           3,4 MTT
1,2 (6) !Fm & !Gm            5 demorgan
1,2 (7) !Fm                  6 &E
1,2 (8) (x)(!Fx)             7 UI
```

(ii.)

(a.)

```
(x)(Gx -> !Fx), (x)(Hx -> Gx) => (x)(Fx -> !Hx)
```

(b.)

```
(x)(Fx -> !F'x), (x)(Hx -> F'x) => (x)(Fx -> !Hx)
```

(c.)

```
(x)(Hx -> F'x), (x)(Fx -> !F'x) => (x)(Hx -> !Fx)
```

(d.)

```
(x)(Gx -> F'x), (x)(F'x -> !Hx) => (x)(Gx -> !Hx)
```
