## The existential quantifier

### Ex.1

(a.)

```
1 (1) (x)(Fx -> Gx)         A
2 (2) (∃x)(!Gx)             A
2 (3) !Ga                   A
1 (4) Fa -> Ga              1 UE
1,2 (5) !Fa                 3,4 MTT
1,2 (6) (∃x)(!Fx)           2,3,5 EE
```

(b.)

```
1 (1) (x)(Fx -> Gx & Hx)        A
2 (2) (∃x)(Fx)                  A
2 (3) Fa                        A
1 (4) Fa -> Ga & Ha             1 UE
1,2 (5) Ga & Ha                 3,4 MPP
1,2 (6) Ha                      1,2 &E
1,2 (7) (∃x)(Hx)                2,3,6 EE
```

(c.)

```
1 (1) (x)(Fx v Gx -> Hx)        A
2 (2) (∃x)(!Hx)                 A
2 (3) !Ha                       A
1 (4) Fa v Ga -> Ha             1 UE
1,2 (5) !(Fa v Ga)              3,4 MTT
6 (6) !(!Fa & !Ga)              A
7 (7) !Fa                       A
8 (8) !Ga                       A
7,8 (9) !Fa & !Ga               7,8 &I
6,7,8 (10) !(!Fa & !Ga) & (!Fa & !Ga) 6,9 &I
6,8 (11) !!Fa                   7,10 RAA
6,8 (12) Fa                     11 DN
6,8 (13) Fa v Ga                12 vI
1,2,6,8 (14) !(Fa v Ga) & (Fa v Ga) 6,13 &I
1,2,6 (15) !!Ga                 8,14 RAA
1,2,6 (16) Ga                   15 DN
1,2,6 (17) Fa v Ga              16 vI
1,2,6  (18) !(Fa v Ga) & (Fa v Ga) 6,17 &I
1,2 (19) !!(!Fa & !Ga)          6,18 RAA
1,2 (20) !Fa & !Ga              19 DN
1,2 (21) !Fa                    20 &E
1,2 (22) (∃x)(!Fx)              2,3,21 EE
```

### Ex.2

(i.)

(a.)

```
1 (1) (x)(Gx -> !Hx)             A
2 (2) (∃x)(Fx & Gx)              A
3 (3) Fa & Ga                    A
1 (4) Ga -> !Ha                  1 UE
3 (5) Ga                         3 &E
1,3 (6) !Ha                      4,5 MPP
3 (7) Fa                         3 &E
1,3 (8) Fa & !Ha                 6,7 &I
1,2 (9) (∃x)(Fx & !Hx)           2,3,8 EE
```

(b.)

similar to a., use `MTT`

(c.)

similar to b., add `DN`

(d.), (e.), (f.), (g.)

similar to a.

(ii.)

(a.)

`(x)(Mx -> !Cx), (∃x)(Hx & Cx) => (∃x)(Hx & !Mx)`

(b.)

`(∃x)(Mx & Cx), (x)(Mx -> Hx) => (∃x)(Hx & Cx)`

(c.)

`(x)(Hx -> Cx), (∃x)(Mx & !Cx) => (∃x)(Mx & !Hx)`

(d.)

`(x)(Hx -> Cx), (∃x)(Mx & Hx) => (∃x)(Mx & Cx)`

(e.)

`(x)(Mx -> !Cx), (∃x)(Hx & Mx) => (∃x)(Hx & !Cx)`

(f.)

`(∃x)(Mx & !Cx), (x)(Mx -> Hx) => (∃x)(Hx & !Cx)`

(g.)

`(x)(Mx -> !Cx), (∃x)(Mx & Hx) => (∃x)(Hx & !Cx)`