## Sequents with quantifiers

### Ex.1

(a.)

`(x)(Fx -> Gx) => (x)(!Gx) -> (x)(!Fx)`

```
1 (1) (x)(Fx -> Gx)              A
1 (2) Fa -> Ga                   1 UE
3 (3) (x)(!Gx)                   A
3 (4) !Ga                        3 UE
1,3 (5) !Fa                      2,4 MTT
1,3 (6) (x)(!Fx)                 5 UI
1 (7) (x)(!Gx) -> (x)(!Fx)       3,6 CP
```

(b.)

`(x)(Fx -> Gx) => (∃x)!Gx -> (∃x)!Fx`

```
1 (1) (x)(Fx -> Gx)                A
1 (2) Fa -> Ga                     1 UE
3 (3) (∃x)(!Gx)                    A
3 (4) !Ga                          3 EE
1,3 (5) !Fa                        2,4 MTT
1,3 (6) (∃x)!Fx                    5 EI
1 (7) (∃x)!Gx -> (∃x)!Fx           1,6 CP
```

(c.)

`(∃x)!Fx <=> !(x)Fx`

(i.) `(∃x)!Fx => !(x)Fx`

```
1 (1) (∃x)!Fx                       A
1 (2) !Fa                           1 EE
3 (3) (x)Fx                         A
3 (4) Fa                            3 UE
1,3 (5) !Fa & Fa                    2,4 &I
1 (6) !(x)Fx                        3,5 RAA
```

(ii.) `!(x)Fx => (∃x)!Fx`

```
1 (1) !(x)Fx                        A
1 (2) !(Fa)                         1 UE
1 (3) (∃x)(!Fx)                     2 EI
```

(d.)

(i.) `(x)!Fx <=> !(∃x)(Fx)`

```
1 (1) (x)!Fx                        A
2 (2) (∃x)(Fx)                      A
1 (3) !Fa                           1 UE
2 (4) Fa                            2 EE
1,2 (5) !Fa & Fa                    3,4 &I
1 (6) !(∃x)(Fx)                     2,5 RAA
```

(ii.) `!(∃x)(Fx) => (x)!Fx`

```
1 (1) !(∃x)(Fx)                     A
2 (2) !(x)!Fx                       A
2 (3) !(!Fa)                        2 UI
2 (4) Fa                            3 DN
2 (5) (∃x)(Fx)                      4 EI
1,2 (6) !(∃x)(Fx) & (∃x)(Fx)        1,5 &I
1 (7) !!(x)!Fx                      2,6 RAA
1 (8) (x)!Fx                        7 DN
```

(e.)

(i.) `(x)(Fx -> !Gx) <=> !(∃x)(Fx & Gx)`

```
1 (1) (x)(Fx -> !Gx)                A
1 (2) Fa -> !Ga                     1 UE
1 (3) !Fa v Ga                      use rule
1 (4) !(Fa & Ga)                    use rule
1 (5) !(∃x)(Fx & Gx)                4 EI
```

(ii.) `!(∃x)(Fx & Gx) => (x)(Fx -> !Gx)`

```
1 (1) !(∃x)(Fx & Gx)                 A
2 (2) !(x)(Fx -> !Gx)                A
2 (3) !(Fa -> !Ga)                   2 UE
2 (4) Fa & Ga                        use rule
2 (5) (∃x)(Fx & Gx)                  4 EI
1,2 (6) !(∃x)(Fx & Gx) & (∃x)(Fx & Gx)  1,5 &I
1 (7) !!(x)(Fx -> !Gx)               2,6 RAA
1 (8) (x)(Fx -> !Gx)                 7 DN
```

(f.)

(i.) `(x)(Fx <-> Gx) => (x)(Fx -> Gx) & (x)(Gx -> Fx)`

```
1 (1) (x)(Fx <-> Gx)              A
1 (2) (x)(Fx -> Gx & Gx -> Fx)    expand (1)
1 (3) Fa -> Ga & Ga -> Fa         2 EI
1 (4) Fa -> Ga                    3 &E
1 (5) (x)(Fx -> Gx)               4 UI
1 (6) Ga -> Fa                    3 &E
1 (7) (x)(Gx -> Fx)               6 UI
1 (8) (x)(Fx -> Gx) & (x)(Gx -> Fx)   5,7 &I
```

(ii.) `(x)(Fx -> Gx) & (x)(Gx -> Fx) => (x)(Fx <-> Gx)`

```
1 (1) (x)(Fx -> Gx) & (x)(Gx -> Fx)     A
1 (2) (x)(Fx -> Gx)                     1 &E
1 (3) (x)(Gx -> Fx)                     1 &E
1 (4) Fa -> Ga                          2 UE
1 (5) Ga -> Fa                          3 UE
1 (6) Fa <=> Ga                         4,5 &I
1 (7) (x)(Fx <=> Gx)                    6 UI
```

(g.)

`(x)(Fx <-> Gx) => (x)(Fx) <-> (x)(Gx)`

```
1 (1) (x)(Fx <-> Gx)                        A
1 (2) (x)(Fx -> Gx & Gx -> Fx)              expand (1)
1 (3) Fa -> Ga & Ga -> Fa                   2 UE
4 (4) (x)(Fx)                               A
4 (5) Fa                                    4 UE
1 (6) Fa -> Ga                              3 &E
1,4 (7) Ga                                  5,6 MPP
1,4 (8) (x)(Gx)                             7 UI
1 (9) (x)(Fx) -> (x)(Gx)                    5,8 CP
similar to how we reach (9), we get the other one
```

(h.)

`(x)(Fx <-> Gx) => (∃x)Fx <-> (∃x)Gx`

```
1 (1) (x)(Fx <-> Gx)                       A
1 (2) (x)(Fx -> Gx & Gx -> Fx)             expand (1)
1 (3) Fa -> Ga & Ga -> Fa                  2 UE
4 (4) (∃x)(Fx)                             A
4 (5) Fa                                   4 EE
1 (6) Fa -> Ga                             3 &E
1,4 (7) Ga                                 5,6 MPP
1,4 (8) (∃x)Gx                             7 EI
1 (9) (∃x)Fx -> (∃x)Gx                     4,8 CP
similar to how reach (9), we get the other one
```

### Ex.2

(i.)

`(x)(Wx -> Fx) <=> !(∃x)(Wx & !Fx)`

```
1 (1) (x)(Wx -> Fx)                 A
2 (2) (∃x)(Wx & !Fx)                A
2 (3) Wa & !Fa                      2 EE
2 (4) !(!Wa v Fa)                   use rule
2 (5) !(Wa -> Fa)                   use rule
1 (6) Wa -> Fa                      1 UE
1,2 (7) !(Wa -> Fa) & (Wa -> Fa)    5,6 &I
1 (8) !(∃x)(Wx & !Fx)               2,7 RAA
```

```
1 (1) !(∃x)(Wx & !Fx)               A
2 (2) !(x)(Wx -> Fx)                A
2 (3) !(Wa -> Fa)                   2 UE
2 (4) Wa & !Fa                      use rule
2 (5) (∃x)(Wx & !Fx)                4 EI
1,2 (6) !(∃x)(Wx & !Fx) & (∃x)(Wx & !Fx)  1,5 &I
1 (7) !!(x)(Wx -> Fx)               2,6 RAA
1 (8) (x)(Wx -> Fx)                 7 DN
```

(ii.)

`(x)(Mx -> Fx) <=> !(∃x)(Mx & !Fx)`

### Ex.3

(a.)

(i.) `(x)(P -> Fx) => P -> (x)(Fx)`

```
1 (1) (x)(P -> Fx)                 A
1 (2) P -> Fa                      1 UE
3 (3) P                            A
1,3 (4) Fa                         2,3 MPP
1,3 (5) (x)(Fx)                    4 UI
1 (6) P -> (x)(Fx)                 3,5 CP
```

(ii.)

```
1 (1) P -> (x)(Fx)                 A
2 (2) P                            A
1,2 (3) (x)(Fx)                    1,2 MPP
1,2 (4) Fa                         3 UE
1 (5) P -> Fa                      2,4 CP
1 (6) (x)(P -> Fx)                 5 UI
```

(b.)

`(x)(P & Fx) <=> P & (x)Fx`

```
1 (1) (x)(P & Fx)                   A
1 (2) P & Fa                        1 UE
1 (3) P                             2 &E
1 (4) Fa                            2 &E
1 (5) (x)(Fx)                       4 UI
1 (6) P & (x)(Fx)                   3,5 &I
```

```
1 (1) P & (x)Fx                     A
1 (2) (x)Fx                         1 &E
1 (3) P                             1 &E
1 (4) Fa                            2 UE
1 (5) P & Fa                        3,4 &I
1 (6) (x)(P & Fx)                   5 UI
```

(c.)

`(∃x)(P & Fx) <=> P & (∃x)Fx`

similar to b.

(d.)

`(x)(P v Fx) <=> P v (x)Fx`

```
1 (1) (x)(P v Fx)               A
1 (2) P v Fa                    1 UE
3 (3) !(P v (x)Fx)              A
3 (4) !P & !(x)Fx               3 use rule
3 (5) !P                        4 &E
3 (6) !(x)Fx                    4 &E
7 (7) P                         A
3,7 (8) !P & P                  5,7 &I
7 (9) !!(P v (x)Fx)             3,8 RAA
10 (10) Fa                      A
3 (11) !Fa                      6 UE
3,10 (12) Fa & !Fa              10,11 &I
10 (13) !!(P v (x)Fx)           3,12 RAA
1 (14) !!(P v (x)Fx)            2,7,9,10,13 vE
1 (15) P v (x)Fx                14 DN
```

```
1 (1) P v (x)Fx                 A
2 (2) P                         A
2 (3) P v Fa                    2 vI
4 (4) (x)Fx                     A
4 (5) Fa                        4 UE
4 (6) P v Fa                    5 vI
1 (7) P v Fa                    1,2,3,4,6 vE
1 (8) (x)(P v Fx)               7 UI
```

(e.)

`(∃x)(P v Fx) <=> P v (∃x)(Fx)`

```
1 (1) (∃x)(P v Fx)              A
2 (2) P v Fa                    A
3 (3) P                         A
3 (4) P v (∃x)(Fx)              3 vI
5 (5) Fa                        A
5 (6) (∃x)(Fx)                  5 EI
2 (7) P v (∃x)(Fx)              2,3,4,5,6 vE
1 (8) P v (∃x)(Fx)              1,2,7 EE
```

```
1 (1) P v (∃x)(Fx)              A
2 (2) P                         A
2 (3) P v Fa                    2 vI
4 (4) (∃x)(Fx)                  A
5 (5) Fa                        A
5 (6) P v Fa                    5 vI
4 (7) (∃x)(P v Fx)              4,5,6 EE
2 (8) (∃x)(P v Fx)              3 EI
1 (9) (∃x)(P v Fx)              1,2,8,4,7 vE
```

(f.)

`(∃x)(Fx -> P) <=> (x)(Fx) -> P`

```
1 (1) (∃x)(Fx -> P)                A
2 (2) Fa -> P                      A
4 (4) (x)Fx                        A
4 (5) Fa                           4 UE
2,4 (6) P                          2,5 MPP
2 (7) (x)Fx -> P                   4,6 CP
1 (8) (x)Fx -> P                   1,2,7 EE
```

```
1 (1) (x)Fx -> P                   A
2 (2) (x)Fx                        A
2 (3) Fa                           2 UE
1,2 (4) P                          1,2 MPP
1 (5) Fa -> P                      3,4 CP
1 (6) (∃x)(Fx -> P)                5 EI
```