## Conditionals and negation

### EX.1

(a.)

P → (P → Q), P ⊢ Q

```
1 (1) P → (P → Q) A
2 (2) P           A
1,2 (3) P → Q       1,2 MPP
1,2 (4) Q           2,3 MPP
```

(b.)

Q → (P → R), ⌐R, Q ⊢ ⌐P

```
1 (1) Q → (P → R)     A
2 (2) Q               A
1,2 (3) P → R           1,2 MPP
4 (4) ⌐R              A
1,2,4 (5) ⌐P              3,4 MTT
```

(c.)

P → ⌐⌐Q, P ⊢ Q

```
1 (1) P → ⌐⌐Q           A
2 (2) P                 A
1,2 (3) ⌐⌐Q               1,2 MPP
1,2 (4) Q                 3 DN
```

(d.)

⌐⌐Q → P, ⌐P ⊢ ⌐Q

```
1 (1) ⌐⌐Q → P             A
2 (2) ⌐P                  A
1,2 (3) ⌐⌐⌐Q                1,2 MTT
1,2 (4) ⌐Q                  3 DN
```

(e.)

⌐P → ⌐Q, Q ⊢ P

```
1 (1) ⌐P → ⌐Q         A
2 (2) Q               A
2 (3) ⌐⌐Q             2 DN
1,2 (4) ⌐⌐P             1,3 MTT
1,2 (5) P               4 DN
```

(f.)

P → ⌐Q ⊢ Q → ⌐P

```
1 (1) P → ⌐Q         A
2 (2) Q              A
2 (3) ⌐⌐Q            2 DN
1,2 (4) ⌐P           1,3 MTT
1 (5) Q → ⌐P         2,4 CP
```

(g.)

⌐P → Q ⊢ ⌐Q → P

```
1 (1) ⌐P → Q          A
2 (2) ⌐Q              A
1,2 (3) ⌐⌐P           1,2 MTT
1,2 (4) P             3 DN
1 (5) ⌐Q → P          2,4 CP
```

(h.)

⌐P → ⌐Q ⊢ Q → P

```
1 (1) ⌐P → ⌐Q             A
2 (2) Q                   A
1,2 (3) ⌐⌐P               1,2 MTT
1,2 (4) P                 3 DN
1 (5) Q → P               2,4 CP
```

(i.)

P → Q, Q → R ⊢ P → R

```
1 (1) P → Q               A
2 (2) Q → R               A
3 (3) P                   A
1,3 (4) Q                 1,3 MPP
1,2,3 (5) R               2,4 MPP
1,2 (6) P → R             3,5 CP
```

(j.)

P → (Q → R) ⊢ (P → Q) → (P → R)

```
1 (1) P → (Q → R)            A
2 (2) P → Q                  A
3 (3) P                      A
1,3 (4) Q → R                1,3 MPP
2,3 (5) Q                    2,3 MPP
1,2,3 (6) R                  A
1,2 (7) P → R                3,6 CP
1 (8) (P → Q) → (P → R)      2,7 CP
```

(k.)

P → (Q → (R → S)) ⊢ R → (P → (Q → S))

```
1 (1) P → (Q → (R → S))             A
2 (2) P                             A
3 (3) Q                             A
4 (4) R                             A
1,2,3,4 (5) S                       1,2,3,4 MPP
1,2,4 (6) Q → S                     3,5 CP
1,4 (7) P → (Q → S)                 2,6 CP
1 (8) R → (P → (Q → S))             4,7 CP
```

(l.)

P → Q ⊢ (Q → R) → (P → R)

```
1 (1) P → Q                  A
2 (2) Q → R                  A
3 (3) P                      A
1,3 (4) Q                    1,3 MPP
1,2,3 (5) R                  2,4 MPP
1,2 (6) P → R                3,5 CP
1 (7) (Q → R) → (P → R)      2,6 CP
```

(m.)

P ⊢ (P → Q) → Q

```
1 (1) P                        A
2 (2) P → Q                    A
1,2 (3) Q                      1,2 MPP
1 (4) (P → Q) → Q              2,3 CP
```

(n.)

P ⊢ (⌐(Q → R) → P) → (⌐R → ⌐Q)

```
1 (1) P                               A
2 (2) ⌐(Q → R) → ⌐P                   A
1,2 (3) Q → R                         1,2 MTT
4 (4) ⌐R                              A
1,2,4 (5) ⌐Q                          3,4 MTT
1,2 (6) ⌐R → ⌐Q                       4,5 CP
1 (7) (⌐(Q → R) → ⌐P) → (⌐R → ⌐Q)     2,6 CP
```

### EX.2

(a.)

P: an element is a member of [1,3,5]
Q: an element is odd

P → ⌐Q, ⌐P ⊢ Q

wrong: an element is not in [1,3,5], then an element is odd

(b.)

⌐P → ⌐Q, ⌐Q ⊢ ⌐P

P: an element is odd
Q: an element is prime

wrong: an element is not prime, then an element is not odd

(c.)

P → Q ⊢ Q → P

P: an element is prime
Q: an element is odd

wrong: an element is odd, then an element is not prime

### Ex.3
