## Biconditional

### Ex.1

(a.)

Q, P <-> Q => P

```
1 (1) Q                      A
2 (2) (P -> Q) & (Q -> P)    A
2 (3) Q -> P                 2 &E
1,2 (4) P                    1,2 MPP
```

(b.)

P -> Q, Q -> P => P <-> Q

```
1 (1) P -> Q                 A
2 (2) Q -> P                 A
1,2 (3) (P -> Q) & (Q -> P)  1,2 &I
```

(c.)

P <-> Q => !P <-> !Q

```
1 (1) (P -> Q) & (Q -> P)           A
1 (2) P -> Q                        1 &I
1 (3) Q -> P                        1 &I
4 (4) !P                            A
5 (5) !Q                            A
1,4 (6) !Q                          3,4 MTT
1,5 (7) !P                          2,5 MTT
1 (8) !P -> !Q                      4,6 CP
1 (9) !Q -> !P                      5,7 CP
1 (10) !P <-> !Q                    8,9 &I 
```

(d.)

!P <-> !Q =>  P <-> Q

```
1 (1) (!P -> !Q) & (!Q -> !P)         A
1 (2) !P -> !Q                        1 &I
1 (3) !Q -> !P                        1 &I
4 (4) P                               A
5 (5) Q                               A
1,4 (6) !!Q                           3,4 MTT
1,5 (7) !!P                           2,5 MTT
1,4 (8) Q                             6 DN
1,5 (9) Q                             7 DN
1 (10) P -> Q                         4,8 CP
1 (11) Q -> P                         5,9 CP
1 (12) P <-> Q                        8,9 &I 
```

(e.)

(P v Q) <-> P => Q -> P

```
1 (1) (P v Q) -> P              A
2 (2) P -> (P v Q)              A
3 (3) Q                         A
3 (4) P v Q                     3 vI
1,3 (5) P                       1,4 MPP
1 (6) Q -> P                    3,5 CP
```

(f.)

P <-> !Q, Q <-> !R => P <-> R

```
1 (1) P -> !Q          A
2 (2) !Q -> P          A
3 (3) Q -> !R          A
4 (4) !R -> Q          A
5 (5) P                A
1,5 (6) !Q             1,5 CP
1,5,4 (7) !!R          4,6 MTT
1,5,4 (8) R            7 DN
1,4 (9) P -> R         5,8 CP
10 (10) R              A
3,10 (11) !Q           3,10 MTT
2,3,10 (12) P          2,11 CPP
2,3 (13) R -> P        10,12 CP
1,2,3,4 (14) P <-> R   9,13 &I
```

### Ex.2

Def.*: P * Q = !P -> Q

(a.)

!P -> Q => !Q -> P

MTT rule

(b.)

!P -> Q, !P -> R => !P -> (Q & R)

```
1 (1) !P -> Q                A
2 (2) !P -> R                A
3 (3) !P                     A
1,3 (4) Q                    1,3 MPP
2,3 (5) R                    2,3 MPP
1,2,3 (6) Q & R              4,5 &I
1,2 (7) P * (Q & R)          3,6 CP
```

(c.)

P * Q, R * !Q => P * R

```
1 (1) !P -> Q                 A
2 (2) !R -> !Q                A
3 (3) !P                      A
1,3 (4) Q                     1,3 MPP
1,2,3 (5) !!R                 2,4 MTT
1,2,3 (6) R                   5 DN
1,2 (7) P * R                 3,6 CP
```

(d.)

P * P => P

see 1-3.j

(e.)

!P * R, !Q * R, P v Q => R

P -> R, Q -> R, P v Q

use &E rule