## Theorems and derived rules

### Ex.1

(a.)

() => (Q -> R) -> ((P -> Q) -> (P -> R))

```
1 (1) Q -> R                         A
2 (2) P -> Q                         A
3 (3) P                              A
2,3 (4) Q                            2,3 MPP
1,2,3 (5) R                          1,4 MPP
1,2 (6) P -> R                       3,5 CP
1 (7) (P -> Q) -> (P -> R)           2,6 CP
() (8) (Q -> R) -> ((P -> Q) -> (P -> Q))    1,7 CP
```

(b.)

() => P -> (Q -> (P & Q))

```
1 (1) P                        A
2 (2) Q                        A
1,2 (3) P & Q                  1,2 &I
1 (4) Q -> (P & Q)             2,3 CP
() (5) P -> (Q -> (P & Q))     1,4 CP
```

(c.)

() => (P -> R) -> ((Q -> R) -> (P v Q -> R))

```
1 (1) P -> R                    A
2 (2) P                         A
1,2 (3) R                       1,2 CP
2 (4) P v Q                     2 vI
1 (5) P v Q -> R                3,4 CP
1 (6) (Q -> R) -> (P v Q -> R)  use (P => Q -> P) theorem
() (7) (P -> R) -> ((Q -> R) -> (P v Q -> R)   1,6 CP
```

(d.)

() => (P -> Q & !Q) -> !P

```
1 (1) P -> Q & !Q                A
2 (2) P                          A
1,2 (3) Q & !Q                   1,2 MPP
1 (4) !P                         2,3 RAA
() () => (P -> Q & !Q) -> !P     1,4 CP
```

(e.)

() => (!P -> P) -> P

```
1 (1) !P -> P             A
2 (2) !P                  A
1,2 (3) P                 1,2 MPP
1 (4) P                   2,3 RAA
() (5) (!P -> P) -> P     1,4 CP
```

