## Theorems and derived rules

### Ex.1

(a.)

() => (Q -> R) -> ((P -> Q) -> (P -> R))

```
1 (1) Q -> R                         A
2 (2) P -> Q                         A
3 (3) P                              A
2,3 (4) Q                            2,3 MPP
1,2,3 (5) R                          1,4 MPP
1,2 (6) P -> R                       3,5 CP
1 (7) (P -> Q) -> (P -> R)           2,6 CP
() (8) (Q -> R) -> ((P -> Q) -> (P -> Q))    1,7 CP
```

(b.)

() => P -> (Q -> (P & Q))

```
1 (1) P                        A
2 (2) Q                        A
1,2 (3) P & Q                  1,2 &I
1 (4) Q -> (P & Q)             2,3 CP
() (5) P -> (Q -> (P & Q))     1,4 CP
```

(c.)

() => (P -> R) -> ((Q -> R) -> (P v Q -> R))

```
1 (1) P -> R                    A
2 (2) P                         A
1,2 (3) R                       1,2 CP
2 (4) P v Q                     2 vI
1 (5) P v Q -> R                3,4 CP
1 (6) (Q -> R) -> (P v Q -> R)  use (P => Q -> P) theorem
() (7) (P -> R) -> ((Q -> R) -> (P v Q -> R)   1,6 CP
```

(d.)

() => (P -> Q & !Q) -> !P

```
1 (1) P -> Q & !Q                A
2 (2) P                          A
1,2 (3) Q & !Q                   1,2 MPP
1 (4) !P                         2,3 RAA
() () => (P -> Q & !Q) -> !P     1,4 CP
```

(e.)

() => (!P -> P) -> P

```
1 (1) !P -> P             A
2 (2) !P                  A
1,2 (3) P                 1,2 MPP
1 (4) P                   2,3 RAA
() (5) (!P -> P) -> P     1,4 CP
```

### Ex.2

(a.)

Q -> P, Q => P

MPP

(b.)

!!P -> !!!P, !!!!P => !P

R -> S, !S => !P

R: !!P
S: !!!P

**the limitation of using DN**

(c.)

!P & (Q & R) -> Q v P => !P -> (Q & R -> Q v P)

A3 & A1 -> A2 => A3 -> (A1 -> A2)

**ex.13**

(d.)

(!Q -> Q) -> !(!Q -> Q) => !(!Q -> Q)

P -> !P => !P

(e.)

!(S v P) => S v P -> (P & Q <-> R v !S)

!P => P -> ALL_PROPOSITIONAL

### Ex.3

(a.)

() => P -> P v Q

```
1 (1) P                A
1 (2) P v Q            1 vI
() (3) P -> P v Q      1,2 CP
```

(b.)

Q -> P => P v Q <-> P

```
1 (1) Q -> P              A
2 (2) P v Q               A
3 (3) P                   A
4 (4) Q                   A
1,4 (5) P                 1,4 MPP
1,2 (6) P                 2,3,3,4,5 vE
1 (7) (P v Q) -> P        2,6 CP
() (8) P -> P v Q         3.a
1 (9) P v Q <-> P         7,8 &I
```

(c.)

P v Q <-> P <=> Q -> P

P v Q <-> P => Q -> P

1.4.1.e

### Ex.4

(a.)

P & Q <=> P & (P <-> Q)

P & Q => P & (P <-> Q)

```
1 (1) P & Q                 A
1 (2) P                     A
1 (3) Q                     A
1 (4) P -> Q                use Q => P -> Q
1 (5) Q -> P                use P => Q -> P
1 (6) P -> Q & Q -> P       4,5 &I
1 (7) P & (P <-> Q)         2,6 &I
```

P & (P <-> Q) => P & Q

```
1 (1) P & (P <-> Q)           A
1 (2) P                       1 &E
1 (3) P -> Q                  1 &E
1 (4) Q                       2,3 MPP
1 (5) P & Q                   2,4 &I
```

### Ex.5

(a.)

() => P v (P -> Q)

```
1 (1) !(P v (P -> Q))         A
1 (2) !P & !(P -> Q)          use demorgan law
1 (3) !P                      2 &E
1 (4) !(P -> Q)               2 &E
1 (5) P -> Q                  3 (!P => P -> Q)
1 (6) !(P -> Q) & (P -> Q)    4,5 &I
() (7) !!(P v (P -> Q))       1,6 RAA
() (8) P v (P -> Q)           7 DN
```

(b.)

() => (P -> Q) v (Q -> R)

```
() (1) P v !P                  A
2 (2) P                        A
2 (3) Q -> P                   use (P => Q -> P)
2 (4) (P -> Q) v (Q -> P)      3 vI
5 (5) !P                       A
5 (6) P -> Q                   use (!P => P -> Q)
5 (7) (P -> Q) v (Q -> P)      6 vI
() (8) (P -> Q) v (Q -> P)     1,2,4,5,7 vE
```

(c.)

() => ((P -> Q) -> P) -> P

```
1 (1) (P -> Q) -> P            A
1 (2) !(P -> Q) v P            use P -> Q => !P v Q
3 (3) !(P -> Q)                A
4 (4) !P                       A
4 (5) P -> Q                   use P => P -> Q
3,4 (6) !(P -> Q) & (P -> Q)   3,5 &I
3 (7) P                        4,6 RAA
8 (8) P                        A
1 (9) P                        2,3,7,7,7 vE
() (10) ((P -> Q) -> P) -> P   1,9 CP
```

(d.)

!Q => P -> (Q -> R)

```
1 (1) !Q                     A
1 (2) Q -> R                 use !Q => Q -> R
1 (3) P -> (Q -> R)          use P => Q -> P
```

(e.)

P, !P => Q

```
1 (1) P                   A
2 (2) !P                  A
2 (3) P -> Q              use !P => P -> Q
1,2 (4) Q                 1,3 MPP
```

(f.)

P v Q <=> !P -> Q

P v Q => !P -> Q

```
1 (1) P v Q                  A
2 (2) P                      A
2 (3) !!P                    2 DN
2 (4) !P -> Q                use !P => P -> Q
5 (5) Q                      A
5 (6) !P -> Q                use P => Q -> P
1 (7) !P -> Q                1,2,4,5,6 vE
```

!P -> Q => P v Q

```
1 (1) !P -> Q                   A
1 (2) !!P v Q                   use P -> Q => !P v Q
3 (3) !!P                       A
3 (4) P                         3 DN
3 (5) P v Q                     4 vI
6 (6) Q                         A
6 (7) P v Q                     6 vI
1 (8) P v Q                     2,3,5,6,7 vE
```

(g.)

!(P -> Q) <=> P & !Q

!(P -> Q) => P & !Q

```
1 (1) !(P -> Q)                   A
2 (2) !(P & !Q)                   A
2 (3) !P v Q                      use demorgan law
2 (4) P -> Q                      use !P v Q => P -> Q
1,2 (5) !(P -> Q) & (P -> Q)      1,4 &I
1 (6) !!(P & !Q)                  2,5 RAA
1 (7) P & !Q                      2,6 RAA
```

P & !Q => !(P -> Q)

```
1 (1) P & !Q                      A
1 (2) P                           1 &E
1 (3) !Q                          1 &E
4 (4) P -> Q                      A
1,4 (5) !P                        3,4 MTT
1,4 (6) P & !P                    2,5 &I
1 (7) !(P -> Q)                   4,6 RAA
```

(h.)

(P -> Q) -> Q <=> P v Q

(P -> Q) -> Q => P v Q

```
1 (1) (P -> Q) -> Q                A
1 (2) !(P -> Q) v Q                use P -> Q => !P v Q
3 (3) !(P -> Q)                    A
3 (4) P & !Q                       use g.
5 (5) P                            4 &E
5 (6) P v Q                        5 vI
7 (7) Q                            A
7 (8) P v Q                        7 vI
1 (9) P v Q                        1,3,5,7,8 vE
```

(i.)

(P -> Q) v (P -> R) <=> P -> Q v R

(P -> Q) v (P -> R) => P -> Q v R

```
1 (1) (P -> Q) v (P -> R)               A
2 (2) P -> Q                            A
3 (3) P                                 A
2,3 (4) Q                               2,3 MPP
2,3 (5) Q v R                           4 vI
2 (6) P -> Q v R                        2,5 CP
7 (7) P -> R                            A
3,7 (8) R                               3,7 MPP
3,7 (9) Q v R                           8 vI
7 (10) P -> Q v R                       3,9 CP
1 (11) P -> Q v R                       1,2,6,8,10 vE
```

P -> Q v R => (P -> Q) v (P -> R)

```
1 (1) P -> Q v R                        A
1 (2) !P v (Q v R)                      use P -> Q => !P v Q
3 (3) !P                                A
3 (4) P -> Q                            use !P => P -> Q
3 (5) (P -> Q) v (P -> R)               vI
6 (6) Q v R                             A
6 (7) Q                                 A
6 (8) P -> Q                            use P => Q -> P
6 (9) (P -> Q) v (P -> R)               8 vI
10 (10) R                               A
10 (11) P -> R                          use R => P -> R
10 (12) (P -> Q) v (P -> R)             11 vI
6 (13) (P -> Q) v (P -> R)              6,7,9,10,12 vE
1 (14) (P -> Q) v (P -> R)              2,3,5,6,13 vE
```

(j.)

P -> Q <=> (P <-> Q) v Q

((P -> Q) & (Q -> P)) v Q

P -> Q => (P <-> Q) v Q

```
1 (1) P -> Q                A
() (2) Q v !Q               theorem
3 (3) Q                     A
3 (4) (P <-> Q) v Q         3 vI
5 (5) !Q                    A
5 (6) Q -> P                use !Q => Q -> P
1,5 (7) (P <-> Q)           1,6 &I
1,5 (8) (P <-> Q) v Q       7 vI
1 (9) (P <-> Q) v Q         2,3,4,5,8 vE
```

(P <-> Q) v Q => P -> Q

```
1 (1) (P <-> Q) v Q            A
2 (2) P <-> Q                  A
2 (3) P -> Q                   2 &E
4 (4) Q                        A
4 (5) P -> Q                   use Q => P -> Q
1 (6) P -> Q                   1,2,3,4,5 vE
```

(k.)

Q => P & Q <-> P

```
1 (1) Q                     A
2 (2) P                     A
1,2 (3) P & Q               1,2 &I
1 (4) P -> P & Q            2,3 CP
3 (5) P & Q                 A
3 (6) P                     5 &E
() (7) P & Q -> P           5,6 CP
1 (8) P & Q <-> P           4,7 &I
```

(l.)

!Q => P v Q <-> P

```
1 (1) !Q                  A
2 (2) P                   A
2 (3) P v Q               2 vI
() (4) P -> P v Q         2,3 CP
5 (5) P v Q               A
5 (6) !P -> Q             use P v Q => !P -> Q
1,5 (7) !!P               1,6 MTT
1,5 (8) P                 7 DN
1 (9) P v Q -> P          5,8 CP
1 (10) P v Q <-> P        4,9 &I
```

### Ex.6

(i.)

supposed A => B is provable

```
1 (1) A             A
1 (2) B             1 SI
() (3) A -> B       1,2 CP
```

then () => A -> B is provable

supposed () => A -> B is provable

```
1 (1) A             A
() (2) A -> B       Theorem
1 (3) B             1,2 MPP
```

then A => B is provable

(ii.)

similar to (i.)

### Ex.7

P => !!P

```
1 (1) P             A
2 (2) !P            A
1,2 (3) P & !P      1,2 &I
1 (4) !!P           2,3 RAA
```
