## Substitution and completeness

### Ex.1

(a.)

101: Fm, (x)(Fx -> !Gx) => !Gm

F: Fx v Hx, G: Hxa

Fm v Fm, (x)(Fx v Hx -> !Hxa) => !(Hma)

(b.)

103: (x)(Fx -> Gx), (x)Fx => (x)Gx

G: (y)Gxy

(x)(Fx -> (y)Gxy), (x)Fx => (x)(y)Gxy

(c.)

104: (x)Fx => (∃x)Fx

F: (∃y)(Fxy v Gya)

(x)(∃y)(Fxy v Gya) => (∃x)(∃y)(Gxy v Gya)

(d.)

109: (x)(Fx & Gx) <=> (x)Fx & (x)Gx

F: Fx -> Hx, G: Hx -> Fx

(x)((Fx -> Hx) & (Hx -> Fx)) <=> (x)(Fx -> Hx) & (x)(Hx -> Fx)

(e.)

116: (∃x)Fx <=> (∃y)Fy

F: (∃z)(Fxz & Gzx)

(∃x)(∃z)(Fxz & Gzx) <=> (∃x)(∃z)(Fxz & Gzx)

(f.)

119: (∃x)(P -> Fx) <=> P -> (∃x)Fx

F: (y)Gyx, P: (z)Gza

(∃x)((z)Gza -> (y)Gyx) <=> (z)Gza -> (∃x)(y)Gyx

(g.)

120: (x)(y)Fxy <=> (y)(x)Fxy

F: (z)Fxyz

(x)(y)(z)Fxyz <=> (y)(x)(z)Fxyz

(h.)

123: (x)(Fx -> Gx) => (x)((∃y)(Fy & Hxy) -> (∃y)(Gy & Hxy))

F: Fxa v (z)Kzx, G: (z)Fzx, H: (z)(Fxz -> Gzy)

(x)((Fxa v (z)Kzx) -> (z)Fzx) => (x)((∃y)((Fya v (z)Kzy) & (z)(Fxz -> Gzy)) -> (∃y)((z)Fzy & (z)(Fxz -> Gzy)))

### Ex.2

(a.)

```
1 (1) (x)Fx & (∃x)Gx          A
1 (2) (x)Fx                   1 &E
1 (3) Fa                      2 UE
1 (4) (∃x)Gx                  1 &E
5 (5) Ga                      A
1,5 (6) Fa & Ga               3,5 &I
1,5 (7) (∃x)(Fx & Gx)         6 EI
1 (8) (∃x)(Fx & Gx)           4,5,7 EE
```

(b.)

```
1 (1) (x)Fx v (∃x)Gx           A
2 (2) (x)Fx                    A
2 (3) Fa                       2 UE
2 (4) Fa v Ga                  3 vI
2 (5) (∃x)(Fx v Gx)            4 EI
6 (6) (∃x)Gx                   A
7 (7) Ga                       A
7 (8) Fa v Ga                  7 vI
7 (9) (∃x)(Fx v Gx)            8 EI
6 (10) (∃x)(Fx v Gx)           6,7,9 EE
1 (11) (∃x)(Fx v Gx)           1,2,6,10, vE
```

(c.)

```
1 (1) (∃x)Fx -> (x)Gx => (x)(Fx -> Gx)      A
2 (2) (∃x)Fx                                A
2 (3) Fa                                    2 UE
1,2 (4) (x)Gx                               1,2 MPP
1,2 (5) Ga                                  4 UE
1 (6) Fa -> Ga                              3,5 CP
1 (7) (x)(Fx -> Gx)                         6 UI
```

(d.)

```
1 (1) (x)(Fx v Gx)              A
1 (2) Fa v Ga                   1 UE
3 (3) Fa                        A
3 (4) (x)Fx                     3 UI
3 (5) (x)Fx v (∃x)Gx            4 vI
6 (6) Ga                        A
6 (7) (∃x)Gx                    6 EI
6 (8) (x)Fx v (∃x)Gx            7 vI
1 (9) (x)Fx v (∃x)Gx            1,2,5,6,8 vE
```

(e.)

```
1 (1) (x)Fx -> (x)Gx                 A
2 (2) (x)Fx                          A
2 (3) Fa                             2 UE
1,2 (4) (x)Gx                        1,2 MPP
1,2 (5) Ga                           4 UE
1 (6) Fa -> Ga                       3,5 CP
1 (7) (∃x)(Fx -> Gx)                 6 EI
```

(f.)

```
1 (1) (∃x)(Fx -> Gx)                A
2 (2) Fa -> Ga                      A
3 (3) (x)Fx                         A
3 (4) Fa                            3 UE
2,3 (5) Ga                          2,4 MPP
2,3 (6) (∃x)Gx                      5 EI
2 (7) (x)Fx -> (∃x)Gx               3,6 CP
1 (8) (x)Fx -> (∃x)Gx               1,2,7 EE
```

### Ex.3

(a.)

```
1 (1) (y)Fy                  A
1 (2) (y)((x)Fx -> Fy)       use P => Q -> P
```

(b.)

```
1 (1) (y)Fy              A
1 (2) Fa                 1 UE
1 (3) (∃x)(Fx)           2 EI
  (4) Fa -> (∃x)(Fx)     2,3 CP
  (5) (y)(Fy -> (∃x)Fx)  4 UI
```

(c.)

```
1 (1) Fa                 A
1 (2) (∃x)Fx             1 EI
  (3) Fa -> (∃x)Fx       1,2 CP
  (4) (∃y)(Fy -> (∃x)Fx) 3 EI
```

(d.)

```
1 (1) Fy                  A
1 (2) (∃x)Fx -> Fy        use P => Q -> P
1 (3) (∃y)((∃x)Fx -> Fy)  2 EI
```

### Ex.4

(a.)

113: (∃x)Fx <=> !(x)!Fx

EI: A(t) => !(v)!A(v)

```
1 (1) A(t)            A
2 (2) (v)!A(v)        A
2 (3) !A(t)           2 UE
1,2 (4) A(t) & !A(t)  2,3 &I
1 (5) !(v)!A(v)       2,4 RAA
```

EE:

```
1 (1) !(v)!A(v)          A
2 (2) A(t)               A
3 (3) A(t) -> P          A
2,3 (4) P                2,3 MPP
5 (5) !P                 A
3,5 (6) !A(t)            3,5 MTT
3,5 (7) (v)!A(v)         6 UI
1,3,5 (8) !(v)!A(v) & (v)!A(v)  1,7 &I
1,3 (9) !!P              5,8 RAA
1,3 (10) P               9 DN
```

(b.)

113: (x)Fx = !(∃x)!Fx

UE:

```
1 (1) !(∃v)!A(v)           A
2 (2) !A(t)                A
2 (3) (∃v)!A(v)            2 EI
1,2 (4) !(∃v)!A(v) & (∃v)!A(v) 1,3 &I
1 (5) !!A(t)               1,4 RAA
1 (6) A(t)                 5 DN
```

UI:

```
1 (1) A(t)                 A
2 (2) (∃v)!A(v)            A
3 (3) !A(t)                A
1,3 (4) A(t) & !A(t)       1,3 &I
1,2 (5) A(t) & !A(t)       2,3,4 EE
1 (6) !(∃v)!A(v)           2,5 RAA 
```