## Identity

### Ex.1

(a.)

`Fa <=> (x)(x = a -> Fx)`

```
1 (1) Fa            A
1 (2) b = a -> Fa   use P => Q -> P
3 (3) (x)(x = a -> Fa) 2 UI
```

```
1 (1) (x)(x = a -> Fx)     A
1 (2) a = a -> Fa          1 UE
  (3) a = a                =U
1 (4) Fa                   2,3 MPP
```

(b.)

```
1 (1) Fa & a = b            A
1 (2) Fa                    1 &E
1 (3) a = b                 1 &E
1 (4) Fb                    2,3 =E
  (5) Fa & a = b -> Fb      1,4 CP
  (6) (x)(y)(Fx & x = y -> Fy)  5 UI
```

(c.)

```
1 (1) b = a                 A
2 (2) c = a                 A
  (3) c = c                 
2 (4) a = c                 2,3 =E
1,2 (5) b = c               1,4 =E
```

(d.)

```
1 (1) a = b            A
2 (2) Fa               A
1,2 (3) Fb             1,2 =E
1 (4) Fa -> Fb         2,3 CP
5 (5) Fb               A
1,5 (6) Fa             1,5 =E
1 (7) Fb -> Fa         5,6 CP
1 (8) Fa <-> Fb        4,7 &I
```

(e.)

```
1 (1) a = b               A
2 (2) c = a               A
1,2 (3) c = b             1,2 =E
1 (4) c = a => c = b      2,3 CP
```

(f.)

```
  (1) a = a          
  (2) (∃x)(x = a)
```

### Ex.2

(a.)

```
1 (1) (x)(Mx -> Ix)          A
2 (2) Mj                     A
3 (3) j = h                  A
1 (4) Mj -> Ij               A
1,2 (5) Ij                   2,4 MPP
1,2,3 (6) Ih                 3,5 =E
```

(b.)

```
1 (1) !(∃x)(Mx & Sx)         A
2 (2) Mj                     A
3 (3) Sh                     A
4 (4) j = h                  A
3,4 (5) Sj                   3,4 =E
2,3,4 (6) Mj & Sj            2,5 &I
2,3,4 (7) (∃x)(Mx & Sx)      6 EI
1,2,3,4 (8) !(∃x)(Mx & Sx) & (∃x)(Mx & Sx)   1,7 &I
1,2,3 (9) !(j = h)           4,8 RAA
```

(c.)

```
1 (1) (x)(Dx -> x = t v x = j)       A
2 (2) Tt & Tj                        A
3 (3) !(x)(Dx -> Tx)                 A
3 (4) !(Da -> Ta)                    3 UE
3 (5) Da & !Ta                       4 demorgan
1 (6) Da -> a = t v a = j            1 UE
3 (7) Da                             5 &E
1,3 (8) a = t v a = j                6,7 MPP
2 (9) Tt                             2 &E
2 (10) Tj                            2 &E
3 (11) !Ta                           5 &E
12 (12) a = t                        A
2,12 (13) Ta                         9,12 =E
2,3,12 (14) !Ta & Ta                 11,13 &I
15 (15) a = j                        A
2,15 (16) Ta                         10,15 =E
2,3,15 (17) !Ta & Ta                 11,16 &I
1,2,3 (18) !Ta & Ta                  8,12,14,15,17 vE
1,2 (19) !!(x)(Dx -> Tx)             3,18 RAA
1,2 (20) (x)(Dx -> Tx)               19 DN
```

(d.)

```
1 (1) (x)(Ux -> (y)(Uy -> x = y))        A
2 (2) Um                                 A
3 (3) !(j = m)                           A
4 (4) Uj                                 A
1 (5) Uj -> (y)(Uy -> j = y)             1 UE
1,4 (6) (y)(Uy -> j = y)                 4,5 MPP
1,4 (7) Um -> j = m                      6 UE
1,2,4 (8) j = m                          6,7 MPP
1,2,3,4 (9) !(j = m) & (j = m)           3,8 &I
1,2,3 (10) !Uj                           4,9 RAA
```

### Ex.3

(a.)

`(∃x)(Fx & (y)(Fy -> x = y)) <=> (∃x)Fx & (x)(y)(Fx & Fy -> x = y)`

```
1 (1) (∃x)(Fx & (y)(Fy -> x = y))          A
2 (2) Fa & (y)(Fy -> a = y)                A
2 (3) Fa                                   2 &E
2 (4) (y)(Fy -> a = y)                     2 &E
2 (5) (∃x)Fx                               3 EI
2 (6) Fb -> a = b                          4 UE
2 (7) Fa & Fb -> a = b                     use P, Q -> R => P & Q -> R
2 (8) (y)(Fa & Fy -> a = y)                7 UI
1 (9) (y)(Fa & Fy -> a = y)                1,2,8 EE
1 (10) (x)(y)(Fx & Fy -> x = y)            9 UI
1 (11) (∃x)Fx                              1,2,5 EE
1 (12) (∃x)Fx & (x)(y)(Fx & Fy -> x = y)   10,11 &I
```

(b.)

```
1 (1) (∃x)Fx & (x)(y)(Fx & Fy -> x = y)     A
1 (2) (∃x)Fx                                1 &E
1 (3) (x)(y)(Fx & Fy -> x = y)              1 &E
2 (4) Fa                                    A
1 (5) (y)(Fa & Fy -> a = y)                 3 UE
1 (6) Fa & Fc -> a = c                      5 UE
1,2 (7) Fc -> a = c                         use P, Q & P -> R => Q -> R
1,2 (8) (y)(Fy -> a = y)                    7 UI
1,2 (9) Fa & (y)(Fy -> a = y)               4,8 &I
1,2 (10) (∃x)(Fx & (y)(Fy -> x = y))        9 EI
```

### Ex.4

(a.)

```
(x)(Fx -> (y)(Fy -> (z)(Fz -> z = x v z = y)))
```

(b.)

```
(∃x)(Fx &
  (∃y)(Fy & !(x = y) &
    (∃z)(Fz & !(z = x) & !(z = y) &
      (u)(Fu -> u = x v u = y v u = z)
    )
  )
)
```

### Ex.5

```
1 (1) (∃x)(Ax & Dx & (y)(Ay -> x = y))            A
2 (2) Ah                                          A
3 (3) Am & Dm & (y)(Ay -> m = y)                  A
3 (4) Am & Dm                                     3 &E
3 (5) Ah -> m = h                                 A
2,3 (6) m = h                                     2,5 MPP
3 (7) Dm                                          4 &E
2,3 (8) Dh                                        6,7 =E
1,2 (9) Dh                                        1,3,8 EE
```